{
 "cells": [
  {
   "cell_type": "markdown",
   "id": "be2e2778-b6c3-4f8e-8b36-dd6a97ef7529",
   "metadata": {},
   "source": [
    "# Symbolic verification for PRP method (using the Wolfram Language)"
   ]
  },
  {
   "cell_type": "markdown",
   "id": "55b4c4d8-4502-4b15-bb8f-d899ab28af5a",
   "metadata": {},
   "source": [
    "This notebook provides a symbolic verification of the technical statement of Lemma 2.1 of the paper, which can be stated as follows.\n",
    "\n",
    "### Lemma 2.1\n",
    "Let\n",
    "$f\\in\\mathcal{F}_{\\mu,L}$, and let $x_{k-1},d_{k-1}\\in\\mathbb{R}^{n}$\n",
    "and $x_{k}$, $d_{k}$ be generated by the {\\PRP} method (i.e., $\\eta=1$). It holds that: \n",
    "\\begin{equation}\n",
    "\\frac{\\|d_{k}\\|^{2}}{\\|\\nabla f(x_{k})\\|^{2}}\\leq\\frac{(1+q)^{2}}{4q},\\label{eq:PRP_angle}\n",
    "\\end{equation}\n",
    "with $q\\triangleq\\frac{\\mu}{L}$. Equivalently, $\\|d_{k}-\\nabla f(x_{k})\\|\\leq\\epsilon\\|\\nabla f(x_{k})\\|$\n",
    "holds with $\\epsilon=\\frac{1-q}{1+q}$. \n",
    "\n",
    "### Proof\n",
    "\n",
    "Recall that $x_{k}=x_{k-1}-\\gamma_{k-1}\\,d_{k-1}$ and $d_{k}=\\nabla f(x_{k})+\\beta_{k-1}d_{k-1}$.\n",
    "The proof consists of the following weighted sum of inequalities: \n",
    "\n",
    "- optimality condition of the line search, with weight $\\lambda_{1}=-\\beta_{k-1}^{2}\\frac{1+q}{L\\gamma_{k-1}q}$:\n",
    "\n",
    "$$\\langle\\nabla f(x_{k});d_{k-1}\\rangle=0,$$\n",
    "\n",
    "- smoothness and strong convexity of $f$ between $x_{k-1}$ and $x_{k}$,\n",
    "with weight $\\lambda_{2}=\\frac{\\beta_{k-1}^{2}(1+q)^{2}}{L\\gamma_{k-1}^{2}(1-q)q}$:\n",
    "$$\\begin{aligned}f(x_{k-1})\\geq & f(x_{k})+\\langle\\nabla f(x_{k});x_{k-1}-x_{k}\\rangle+\\tfrac{1}{2L}\\|\\nabla f(x_{k-1})-\\nabla f(x_{k})\\|^{2}\\\\\n",
    " & \\quad+\\tfrac{\\mu}{2(1-\\mu/L)}\\|x_{k-1}-x_{k}-\\tfrac{1}{L}(\\nabla f(x_{k-1})-\\nabla f(x_{k}))\\|^{2}\\\\\n",
    "= & f(x_{k})+\\gamma_{k-1}\\langle\\nabla f(x_{k});\\,d_{k-1}\\rangle+\\tfrac{1}{2L}\\|\\nabla f(x_{k-1})-\\nabla f(x_{k})\\|^{2}\\\\\n",
    " & \\quad+\\tfrac{\\mu}{2(1-\\mu/L)}\\|\\gamma_{k-1}d_{k-1}-\\tfrac{1}{L}(\\nabla f(x_{k-1})-\\nabla f(x_{k}))\\|^{2}\n",
    "\\end{aligned}$$\n",
    "\n",
    "- smoothness and strong convexity of $f$ between $x_{k}$ and $x_{k-1}$,\n",
    "with weight $\\lambda_{3}=\\lambda_{2}$: \n",
    "$$\n",
    "\\begin{aligned}f(x_{k})\\geq & f(x_{k-1})+\\langle\\nabla f(x_{k-1});\\,x_{k}-x_{k-1}\\rangle+\\tfrac{1}{2L}\\|\\nabla f(x_{k-1})-\\nabla f(x_{k})\\|^{2}\\\\\n",
    " & \\quad+\\tfrac{\\mu}{2(1-\\mu/L)}\\|x_{k-1}-x_{k}-\\tfrac{1}{L}(\\nabla f(x_{k-1})-\\nabla f(x_{k}))\\|^{2}\\\\\n",
    "= & f(x_{k-1})-\\gamma_{k-1}\\langle\\nabla f(x_{k-1}),d_{k-1}\\rangle+\\tfrac{1}{2L}\\|\\nabla f(x_{k-1})-\\nabla f(x_{k})\\|^{2}\\\\\n",
    " & \\quad+\\tfrac{\\mu}{2(1-\\mu/L)}\\|\\gamma_{k-1}d_{k-1}-\\tfrac{1}{L}(\\nabla f(x_{k-1})-\\nabla f(x_{k}))\\|^{2}\n",
    "\\end{aligned}\n",
    "$$\n",
    "\n",
    "- definition of $\\beta_{k-1}$ with weight $\\lambda_{4}=\\frac{\\beta_{k-1}(1+q)}{L\\gamma_{k-1}q}$:\n",
    "$$\n",
    "\\begin{aligned}0 & =\\langle\\nabla f(x_{k-1});\\,\\nabla f(x_{k})\\rangle-\\|\\nabla f(x_{k})\\|^{2}+\\beta_{k-1}\\|\\nabla f(x_{k-1})\\|^{2}\\\\\n",
    " & =\\langle\\nabla f(x_{k-1});\\,\\nabla f(x_{k})\\rangle-\\|\\nabla f(x_{k})\\|^{2}+\\beta_{k-1}\\langle\\nabla f(x_{k-1});\\,d_{k-1}\\rangle.\n",
    "\\end{aligned}\n",
    "$$\n",
    "\n",
    "\n",
    "We arrive to the following weighted sum: \n",
    "$$\n",
    "\\begin{aligned}0\\geq & \\lambda_{1}\\langle\\nabla f(x_{k});d_{k-1}\\rangle\\\\\n",
    " & +\\lambda_{2}\\bigg[f(x_{k})-f(x_{k-1})+\\gamma_{k-1}\\langle\\nabla f(x_{k});\\,d_{k-1}\\rangle+\\tfrac{1}{2L}\\|\\nabla f(x_{k-1})-\\nabla f(x_{k})\\|^{2}\\\\\n",
    " & \\quad\\quad\\quad+\\tfrac{\\mu}{2(1-\\mu/L)}\\|\\gamma_{k-1}d_{k-1}-\\tfrac{1}{L}(\\nabla f(x_{k-1})-\\nabla f(x_{k}))\\|^{2}\\bigg]\\\\\n",
    " & +\\lambda_{3}\\bigg[f(x_{k-1})-f(x_{k})-\\gamma_{k-1}\\langle\\nabla f(x_{k-1});\\,d_{k-1}\\rangle+\\tfrac{1}{2L}\\|\\nabla f(x_{k-1})-\\nabla f(x_{k})\\|^{2}\\\\\n",
    " & \\quad\\quad\\quad+\\tfrac{\\mu}{2(1-\\mu/L)}\\|\\gamma_{k-1}d_{k-1}-\\tfrac{1}{L}(\\nabla f(x_{k-1})-\\nabla f(x_{k}))\\|^{2}\\bigg]\\\\\n",
    " & +\\lambda_{4}\\big[\\langle\\nabla f(x_{k-1});\\,\\nabla f(x_{k})\\rangle-\\|\\nabla f(x_{k})\\|^{2}+\\beta_{k-1}\\langle\\nabla f(x_{k-1});\\,d_{k-1}\\rangle\\big]\n",
    "\\end{aligned}\n",
    "$$\n",
    "which can be reformulated exactly as (expand both expressions and\n",
    "observe that all terms match---this is done symbolically below) \n",
    "$$\n",
    "\\begin{aligned}0\\geq & \\|d_{k}\\|^{2}-\\frac{(1+q)^{2}}{4q}\\|\\nabla f(x_{k})\\|^{2}\\\\\n",
    " & \\quad+\\frac{4\\beta_{k-1}^{2}q}{(1-q)^{2}}\\left\\Vert d_{k-1}-\\tfrac{1+q}{2L\\gamma_{k-1}q}\\nabla f(x_{k-1})+\\tfrac{2\\beta_{k-1}(1+q)-L\\gamma_{k-1}(1-)^{2}}{4\\beta_{k-1}L\\gamma_{k-1}q}\\nabla f(x_{k})\\right\\Vert ^{2},\n",
    "\\end{aligned}\n",
    "$$\n",
    "the remaining part is provided in the main text.\n",
    "\n",
    "The following symbolic code verifies the equivalence between the weighted sum and its reformulation (referred to as \"target\" hereafter).\n",
    "\n",
    "### Symbolical verification"
   ]
  },
  {
   "cell_type": "code",
   "execution_count": 1,
   "id": "1ced04c3-16ab-46b8-886f-86774c93d8cc",
   "metadata": {},
   "outputs": [
    {
     "ename": "Remove::rmnsm",
     "evalue": "There are no symbols matching \"Global`*\".",
     "output_type": "error",
     "traceback": [
      "\u001b[0;31mRemove::rmnsm: There are no symbols matching \"Global`*\".\u001b[0m"
     ]
    }
   ],
   "source": [
    "(*Clear memory and all the variables*)\n",
    "ClearAll[\"Global`*\"];\n",
    "Remove[\"Global`*\"];\n",
    "SetOptions[EvaluationNotebook[], \n",
    "  CellEpilog :> SelectionMove[EvaluationNotebook[], Next, Cell]];\n",
    "SetOptions[$FrontEnd, \"FileChangeProtection\" -> None];\n",
    "(*You may get the warning:\n",
    "\"Remove::rmnsm: There are no symbols matching \"Global`*\".\"\n",
    "if you run this block twice,\n",
    "but that is fine\n",
    "*)"
   ]
  },
  {
   "cell_type": "code",
   "execution_count": 7,
   "id": "9a7c76ff-9fbb-47fa-8df9-f2e746eb58fa",
   "metadata": {},
   "outputs": [
    {
     "data": {
      "text/html": [
       "<div><pre style=\"&#102;&#111;&#110;&#116;&#45;&#102;&#97;&#109;&#105;&#108;&#121;&#58;&#32;&#34;&#67;&#111;&#117;&#114;&#105;&#101;&#114;&#32;&#78;&#101;&#119;&#34;&#44;&#67;&#111;&#117;&#114;&#105;&#101;&#114;&#44;&#109;&#111;&#110;&#111;&#115;&#112;&#97;&#99;&#101;&#59;\">&#48;</pre></div>"
      ],
      "text/plain": [
       "0"
      ]
     },
     "execution_count": 46,
     "metadata": {
      "text/html": [],
      "text/plain": []
     },
     "output_type": "execute_result"
    }
   ],
   "source": [
    "(* For notational convenience, in the code we let c[k-1] ≜ c, β[k-1] ≜ β, γ[k-1] ≜ γ*)\n",
    "\n",
    "(* System of NCGM *)\n",
    "(* ============== *)\n",
    "\n",
    "d[k] = g[k] + β d[k - 1];\n",
    "\n",
    "x[k] = x[k - 1] - γ d[k - 1];\n",
    "\n",
    "(* Constraints in consideration *)\n",
    "(* ============================ *)\n",
    "\n",
    "\n",
    "constraint1 = g[k] d[k - 1] (* == 0*); \n",
    "\n",
    "constraint2 = \n",
    "  f[k] - f[k - 1] + γ g[k] d[k - 1] + (g[k - 1] - g[k])^2/(\n",
    "   2 L) + (μ (γ d[k - 1] - (g[k - 1] - g[k])/L)^2)/(\n",
    "   2 (1 - μ/L)) (* <= 0*);\n",
    "   \n",
    "constraint3 = \n",
    "  f[k - 1] - f[k] - γ g[k - 1] d[k - 1] + (g[k - 1] - g[k])^2/(\n",
    "   2 L) + (μ (γ d[k - 1] - (g[k - 1] - g[k])/L)^2)/(\n",
    "   2 (1 - μ/L)) (* <= 0*);\n",
    "\n",
    "constraint4 = g[k-1] g[k] - g[k]^2 + β g[k-1] d[k-1]  (* == 0*);\n",
    "\n",
    "   \n",
    "(* Weight λ\"i\" for constraint\"i\" *)   \n",
    "(* ============================ *)\n",
    "\n",
    "q = μ/L;\n",
    "   \n",
    "λ1 = - (β^2 (1+ q)) / (L γ q);\n",
    "    \n",
    "λ2 = (β^2 (1 + q)^2) / (L γ^2 (1 - q) q);\n",
    "\n",
    "λ3 = (β^2 (1 + q)^2) / (L γ^2 (1 - q) q);\n",
    "\n",
    "λ4 = (β (1 + q))/(L γ q);\n",
    "\n",
    "(* Weighted sum *)   \n",
    "(* ==============*)\n",
    "\n",
    "WeightedSum = ((λ1*constraint1) + (λ2*\n",
    "       constraint2) + (λ3*constraint3) + (λ4*\n",
    "       constraint4) // FullSimplify);\n",
    "       \n",
    "(* Target expresion*)   \n",
    "(* ================*)   \n",
    "\n",
    "ν = (1 + (μ/L))^2 / (4 (μ/L));\n",
    "   \n",
    "a1 = (4 β^2 (μ/L)) / (1-(μ/L))^2;\n",
    "\n",
    "a2 = 1;\n",
    "\n",
    "a3 = -( ( 1+(μ/L) ) / (2 L γ (μ/L)) );\n",
    "\n",
    "a4 = ( (2 β (1 + (μ/L))) - L γ (1 - (μ/L))^2 ) / ( 4 β L γ (μ/L) );\n",
    "\n",
    "positiveTerm1 = a1 ( a2 d[k - 1] +  a3 g[k - 1] + a4 g[k] )^2;\n",
    "\n",
    "restTerm2 = -ν g[k]^2 + d[k]^2;\n",
    "\n",
    "SimplifiedTerm = \n",
    " Assuming[β > 0 && c > 1, \n",
    "   Simplify[(positiveTerm1 + restTerm2)]]//Expand;\n",
    "   \n",
    "(* See if both term matches *)\n",
    "TermDiff = Assuming[β > 0 && c > 1 && μ>0 && μ<L, \n",
    " Simplify[WeightedSum - SimplifiedTerm]]   "
   ]
  },
  {
   "cell_type": "code",
   "execution_count": null,
   "id": "cc947441-41f3-458b-b60c-138fdc10811f",
   "metadata": {},
   "outputs": [],
   "source": []
  }
 ],
 "metadata": {
  "kernelspec": {
   "display_name": "Wolfram Language 13.3",
   "language": "Wolfram Language",
   "name": "wolframlanguage13.3"
  },
  "language_info": {
   "codemirror_mode": "mathematica",
   "file_extension": ".m",
   "mimetype": "application/vnd.wolfram.m",
   "name": "Wolfram Language",
   "pygments_lexer": "mathematica",
   "version": "12.0"
  }
 },
 "nbformat": 4,
 "nbformat_minor": 5
}
