{
 "cells": [
  {
   "cell_type": "code",
   "execution_count": 1,
   "id": "ecc9c5ef-f562-4e92-97ca-a105ea1214bb",
   "metadata": {},
   "outputs": [
    {
     "name": "stdout",
     "output_type": "stream",
     "text": [
      "Requirement already satisfied: Sympy in c:\\users\\shuvo\\appdata\\roaming\\jupyterlab-desktop\\jlab_server\\lib\\site-packages (1.12)\n",
      "Requirement already satisfied: mpmath>=0.19 in c:\\users\\shuvo\\appdata\\roaming\\jupyterlab-desktop\\jlab_server\\lib\\site-packages (from Sympy) (1.3.0)\n"
     ]
    }
   ],
   "source": [
    "!pip install Sympy"
   ]
  },
  {
   "cell_type": "markdown",
   "id": "7ee80040-8c6e-473f-81c9-6d0d43acc4c9",
   "metadata": {},
   "source": [
    "# Symbolic verification for FR method (using Sympy)\n",
    "\n",
    "This notebook provides a symbolic verification of the technical statements of Lemma 2.2 and Lemma 2.3 of the paper, which can be stated as follows.\n",
    "\n",
    "### Lemma 2.2\n",
    "\n",
    " Let $f\\in\\mathcal{F}_{\\mu,L}$, and let $x_{k-1},d_{k-1}\\in\\mathbb{R}^{n}$\n",
    "and $x_{k}$, $d_{k}$ be generated by the {\\FR} method (i.e., $\\eta=0$). For any $c_{k-1}\\in\\mathbb{R}$ such that $\\frac{\\|d_{k-1}\\|^{2}}{\\|\\nabla f(x_{k-1})\\|^{2}}=c_{k-1}$,\n",
    "where $c_{k-1}>1$, it holds that: \n",
    "\\begin{equation}\n",
    "0\\leq\\beta_{k-1}\\leq\\frac{1}{c_{k-1}}\\frac{\\left(1-q+2\\sqrt{(c_{k-1}-1)q}\\right)^{2}}{4q},\\label{eq:case_2_beta_FR}\n",
    "\\end{equation}\n",
    "where $q \\triangleq \\frac{\\mu}{L}$.\n",
    "\n",
    "### Proof\n",
    "\n",
    "First, note that $\\beta_{k-1}\\geq0$ by definition. The other part of the proof consists of the following\n",
    "weighted sum of inequalities:\n",
    "\n",
    "- relation between $\\nabla f(x_{k-1})$ and $d_{k-1}$ with weight\n",
    "$\\lambda_{1}=\\gamma_{k-1}(L+\\mu)-\\frac{2\\sqrt{\\beta_{k-1}}}{\\sqrt{(c_{k-1}-1)c_{k-1}}}$: \n",
    "$$\n",
    "0=\\left\\langle \\nabla f(x_{k-1});\\,d_{k-1}\\right\\rangle -\\|\\nabla f(x_{k-1})\\|^{2},\n",
    "$$\n",
    "- optimality condition of the line search with weight $\\lambda_{2}=\\frac{2}{c_{k-1}}-\\gamma_{k-1}(L+\\mu)$: \n",
    "\n",
    "$$0=\\left\\langle \\nabla f(x_{k});\\,d_{k-1}\\right\\rangle ,$$\n",
    "\n",
    "- definition of $\\beta_{k-1}$ with weight $\\lambda_{3}=\\frac{\\sqrt{c_{k-1}-1}}{\\sqrt{\\beta_{k-1}c_{k-1}}}$: \n",
    "$$0=\\|\\nabla f(x_{k})\\|^{2}-\\beta_{k-1}\\|\\nabla f(x_{k-1})\\|^{2},$$\n",
    "\n",
    "- initial condition on the ratio $\\frac{\\|d_{k-1}\\|^{2}}{\\|\\nabla f(x_{k-1})\\|^{2}}$\n",
    "with weight $\\lambda_{4}=-\\gamma_{k-1}^{2}L \\mu +\\frac{\\sqrt{\\beta_{k-1}}}{c_{k-1}\\sqrt{(c_{k-1}-1)c_{k-1}}}$\n",
    ": \n",
    "$$\n",
    "0=\\|d_{k-1}\\|^{2}-c_{k-1}\\|g_{k-1}\\|^{2}$$\n",
    "\n",
    "- smoothness and strong convexity of $f$ between $x_{k-1}$ and $x_{k}$,\n",
    "with weight $\\lambda_{5}=L-\\mu$: \n",
    "\n",
    "$$\\begin{aligned}0\\geq & -f(x_{k-1})+f(x_{k})+\\langle\\nabla f(x_{k});\\,x_{k-1}-x_{k}\\rangle+\\tfrac{1}{2L}\\|\\nabla f(x_{k-1})-\\nabla f(x_{k})\\|^{2}\\\\\n",
    " & \\quad+\\tfrac{\\mu}{2(1-\\mu/L)}\\|x_{k-1}-x_{k}-\\tfrac{1}{L}(\\nabla f(x_{k-1})-\\nabla f(x_{k}))\\|^{2}\\\\\n",
    "= & f(x_{k})+\\gamma_{k-1}\\langle\\nabla f(x_{k});\\,d_{k-1}\\rangle+\\tfrac{1}{2L}\\|\\nabla f(x_{k-1})-\\nabla f(x_{k})\\|^{2}\\\\\n",
    " & \\quad+\\tfrac{\\mu}{2(1-\\mu/L)}\\|\\gamma_{k-1}d_{k-1}-\\tfrac{1}{L}(\\nabla f(x_{k-1})-\\nabla f(x_{k}))\\|^{2}\n",
    "\\end{aligned}$$\n",
    "\n",
    "- smoothness and strong convexity of $f$ between $x_{k}$ and $x_{k-1}$, with weight $\\lambda_{6}=\\lambda_{5}$: \n",
    "\n",
    "$$\\begin{aligned}0\\geq & -f(x_{k})+f(x_{k-1})+\\langle\\nabla f(x_{k-1});\\,x_{k}-x_{k-1}\\rangle+\\tfrac{1}{2L}\\|\\nabla f(x_{k-1})-\\nabla f(x_{k})\\|^{2}\\\\\n",
    " & \\quad+\\tfrac{\\mu}{2(1-\\mu/L)}\\|x_{k-1}-x_{k}-\\tfrac{1}{L}(\\nabla f(x_{k-1})-\\nabla f(x_{k}))\\|^{2}\\\\\n",
    "= & f(x_{k-1})-\\gamma_{k-1}\\langle\\nabla f(x_{k-1});\\,d_{k-1}\\rangle+\\tfrac{1}{2L}\\|\\nabla f(x_{k-1})-\\nabla f(x_{k})\\|^{2}\\\\\n",
    " & \\quad+\\tfrac{\\mu}{2(1-\\mu/L)}\\|\\gamma_{k-1}d_{k-1}-\\tfrac{1}{L}(\\nabla f(x_{k-1})-\\nabla f(x_{k}))\\|^{2}\n",
    "\\end{aligned}$$\n",
    "\n",
    "\n",
    "The weighted sum can be written as: \n",
    "$$\\begin{aligned}\n",
    "0 & \\geq\\lambda_{1}\\left[\\left\\langle \\nabla f(x_{k-1});\\,d_{k-1}\\right\\rangle -\\|\\nabla f(x_{k-1})\\|^{2}\\right]+\\lambda_{2}\\left[\\left\\langle \\nabla f(x_{k});\\,d_{k-1}\\right\\rangle \\right]\\\\\n",
    " & +\\lambda_{3}\\left[\\|\\nabla f(x_{k})\\|^{2}-\\beta_{k-1}\\|\\nabla f(x_{k-1})\\|^{2}\\right]+\\lambda_{4}\\left[\\|d_{k-1}\\|^{2}-c_{k-1}\\|g_{k-1}\\|^{2}\\right]\\\\\n",
    " & +\\lambda_{5}\\Big[f(x_{k})+\\gamma_{k-1}\\langle\\nabla f(x_{k});\\,d_{k-1}\\rangle+\\tfrac{1}{2L}\\|\\nabla f(x_{k-1})-\\nabla f(x_{k})\\|^{2}\\\\\n",
    " & \\quad\\quad+\\tfrac{\\mu}{2(1-\\mu/L)}\\|\\gamma_{k-1}d_{k-1}-\\tfrac{1}{L}(\\nabla f(x_{k-1})-\\nabla f(x_{k}))\\|^{2}\\Big]\\\\\n",
    " & +\\lambda_{6}\\Big[f(x_{k-1})-\\gamma_{k-1}\\langle\\nabla f(x_{k-1});\\,d_{k-1}\\rangle+\\tfrac{1}{2L}\\|\\nabla f(x_{k-1})-\\nabla f(x_{k})\\|^{2}\\\\\n",
    " & \\quad\\quad+\\tfrac{\\mu}{2(1-\\mu/L)}\\|\\gamma_{k-1}d_{k-1}-\\tfrac{1}{L}(\\nabla f(x_{k-1})-\\nabla f(x_{k}))\\|^{2}\\Big],\n",
    "\\end{aligned}$$\n",
    "\n",
    "which can be reformulated exactly as (expand both expressions and\n",
    "observe that all terms match---this is done symbolically below):\n",
    "\n",
    "$$\\begin{align*}\n",
    "0\\geq & \\|\\nabla f(x_{k})\\|^{2}-\\nu(\\beta_{k-1},\\gamma_{k-1},c_{k-1},\\mu,L)\\|\\nabla f(x_{k-1})\\|^{2}\\\\\n",
    " & +\\left\\Vert \\sqrt[4]{\\frac{\\beta_{k-1}}{(c_{k-1}-1)c_{k-1}^{3}}}d_{k-1}-\\sqrt[4]{\\frac{\\beta_{k-1}c_{k-1}}{c_{k-1}-1}}\\nabla f(x_{k-1})+\\sqrt[4]{\\frac{c_{k-1}-1}{\\beta_{k-1}c_{k-1}}}\\nabla f(x_{k})\\right\\Vert ^{2}\n",
    "\\end{align*}$$\n",
    "\n",
    "where \n",
    "$$\n",
    "\\nu(\\beta_{k-1},\\gamma_{k-1},c_{k-1},\\mu,L)=2\\sqrt{1-\\frac{1}{c_{k-1}}}\\sqrt{\\beta_{k-1}}-c_{k-1}\\gamma_{k-1}^{2}L\\mu+\\gamma_{k-1}(L+\\mu)-1.\n",
    "$$\n",
    "\n",
    "The remaining parts are provided in the main text. In the sequel, we provide a symbolical verification for this equivalence.\n",
    "\n",
    "### Symbolical verification"
   ]
  },
  {
   "cell_type": "code",
   "execution_count": 2,
   "id": "4f188ebb-a184-4f87-90b1-9a6590bf1c0d",
   "metadata": {},
   "outputs": [
    {
     "data": {
      "text/latex": [
       "$\\displaystyle 0$"
      ],
      "text/plain": [
       "0"
      ]
     },
     "execution_count": 2,
     "metadata": {},
     "output_type": "execute_result"
    }
   ],
   "source": [
    "import sympy as sm\n",
    "\n",
    "# create symbols for the problem parameters:\n",
    "q = sm.Symbol('q', positive=True) # mu/L\n",
    "gamma = sm.Symbol('gamma_{k-1}')\n",
    "beta = sm.Symbol('beta_{k-1}', positive=True)\n",
    "L = sm.Symbol('L', positive=True)\n",
    "mu = L * q\n",
    "\n",
    "# for enforcing c >= 1, we define c = 1 + cm with cm >= 0.\n",
    "cm = sm.Symbol('cm', positive=True)\n",
    "c = 1 + cm\n",
    "\n",
    "# create symbols for the \"primal\" variables:\n",
    "xk = sm.Symbol('x_{k-1}')\n",
    "gk = sm.Symbol('g_{k-1}')\n",
    "fk = sm.Symbol('f_{k-1}')\n",
    "dk = sm.Symbol('d_{k-1}')\n",
    "gk1 = sm.Symbol('g_{k}')\n",
    "fk1 = sm.Symbol('f_{k}')\n",
    "\n",
    "dk1 = gk1 + beta * dk # define d_{k+1} using previous symbols\n",
    "xk1 = xk - gamma * dk # define x_{k+1} using previous symbols\n",
    "\n",
    "# inequalities\n",
    "constraint1 = gk*dk - gk**2 ## =0\n",
    "constraint2 = gk1 * dk # == 0\n",
    "constraint3 = gk1**2 - beta * gk**2 # == 0 \n",
    "constraint4 =  dk**2 - c * gk**2 # == 0\n",
    "constraint5 = fk1 - fk + gamma * gk1 * dk + 1/2/L * (gk - gk1)**2 + mu/2/(1-q) * (gamma * dk - 1/L * (gk - gk1))**2 # <= 0\n",
    "constraint6 = fk - fk1 - gamma * gk * dk + 1/2/L * (gk - gk1)**2 + mu/2/(1-q)*(gamma * dk - 1/L * (gk - gk1))**2 # <= 0\n",
    "\n",
    "# multipliers\n",
    "lambda1 = gamma*(mu+L) - 2*sm.sqrt(beta)/sm.sqrt((c-1)*c)\n",
    "lambda2 = (2/c) - gamma*(mu+L)\n",
    "lambda3 = sm.sqrt(c-1)/sm.sqrt(beta*c)\n",
    "lambda4 = - (gamma**2)* mu * L + sm.sqrt(beta)/(c*sm.sqrt((c-1)*c))\n",
    "lambda5 = L-mu\n",
    "lambda6 = L-mu\n",
    "\n",
    "# weighted sum\n",
    "weightedSum = lambda1 * constraint1 + lambda2 * constraint2 + lambda3 * constraint3 + lambda4 * constraint4 + lambda5*constraint5 + lambda6*constraint6\n",
    "weightedSum = sm.expand(weightedSum)\n",
    "\n",
    "# target expression\n",
    "\n",
    "nu = 2*(sm.sqrt(c-1)/sm.sqrt(c))*sm.sqrt(beta) - c*(gamma**2)*mu*L + gamma*(mu+L) - 1\n",
    "coef1 = sm.root(beta/((c-1)*(c**3)),4)\n",
    "coef2 = -sm.root((beta*c)/((c-1)),4)\n",
    "coef3 = (sm.root((c-1)/(beta*c),4))\n",
    "target = sm.expand(gk1 ** 2 - nu * gk**2 + ( (coef1*dk) + (coef2*gk) + (coef3*gk1) )**2)\n",
    "\n",
    "# Verify that WeightedSum - Target == 0\n",
    "sm.simplify(target-weightedSum)"
   ]
  },
  {
   "cell_type": "markdown",
   "id": "12844d34-2aae-4c4d-ac10-de62ead78768",
   "metadata": {},
   "source": [
    "### Lemma 2.3\n",
    "\n",
    "Let $f\\in\\mathcal{F}_{\\mu,L}$, and let $x_{k-1},d_{k-1}\\in\\mathbb{R}^{n}$\n",
    "and $x_{k}$, $d_{k}$ be generated by the {\\FR} method (i.e., $\\eta=0$). For any $c_{k-1}\\in\\mathbb{R}$ such that $\\frac{\\|d_{k-1}\\|^{2}}{\\|\\nabla f(x_{k-1})\\|^{2}}=c_{k-1}$,\n",
    "where $c_{k-1}>1$, it holds that: \n",
    "\\begin{equation}\n",
    "\\frac{\\|d_{k}\\|^{2}}{\\|\\nabla f(x_{k})\\|^{2}}\\leq c_{k}\\triangleq1+\\frac{\\left(1-q+2\\sqrt{(c_{k-1}-1)q}\\right)^{2}}{4q},\\label{eq:FR_angle}\n",
    "\\end{equation}\n",
    "with $q\\triangleq\\frac{\\mu}{L}$. Equivalently, $\\|d_{k}-\\nabla f(x_{k})\\|\\leq\\epsilon\\|\\nabla f(x_{k})\\|$\n",
    "holds with $\\epsilon=\\sqrt{1-\\frac{1}{c_{k}}}$.\n",
    "\n",
    "\n",
    "### Proof\n",
    "\n",
    "The proof consists of the following weighted sum of inequalities: \n",
    "\n",
    "- optimality condition of the line search with weight $\\lambda_{1}=2\\beta_{k-1}$:\n",
    "\n",
    "$$\n",
    "0=\\langle\\nabla f(x_{k});d_{k-1}\\rangle,$$\n",
    "\n",
    "- the quality of the search direction with weight $\\lambda_{2}=\\beta_{k-1}^{2}$:\n",
    "\n",
    "$$0=\\|d_{k-1}\\|^{2}-c_{k-1}\\|\\nabla f(x_{k-1})\\|^{2},$$\n",
    "\n",
    "- definition of $\\beta_{k-1}$ with weight $\\lambda_{3}=-c_{k-1}\\beta_{k-1}$:\n",
    "\n",
    "$$\\begin{aligned}0=\\|\\nabla f(x_{k})\\|^{2}-\\beta_{k-1}\\|\\nabla f(x_{k-1})\\|^{2}.\\end{aligned}$$\n",
    "\n",
    "The weighted sum can be written as \n",
    "$$\n",
    "\\begin{aligned}0= & \\lambda_{1}\\left[\\langle\\nabla f(x_{k});d_{k-1}\\rangle\\right]+\\lambda_{2}\\left[\\|d_{k-1}\\|^{2}-c_{k-1}\\|\\nabla f(x_{k-1})\\|^{2}\\right]+\\lambda_{3}\\left[\\|\\nabla f(x_{k})\\|^{2}-\\beta_{k-1}\\|\\nabla f(x_{k-1})\\|^{2}\\right],\\end{aligned}\n",
    "$$  \n",
    "and can be reformulated exactly as (expand both expressions and\n",
    "observe that all terms match---this is done symbolically below) \n",
    "$$\n",
    "\\begin{aligned}0=\\|d_{k}\\|^{2}-(1+c_{k-1}\\beta_{k-1})\\|\\nabla f(x_{k})\\|^{2}.\n",
    "\\end{aligned}\n",
    "$$\n",
    "\n",
    "The remaining parts are provided in the main text. In the sequel, we provide a symbolical verification for this equivalence.\n",
    "\n",
    "### Symbolical verification"
   ]
  },
  {
   "cell_type": "code",
   "execution_count": 3,
   "id": "6c28f26e-4921-498f-9088-dc64b471bce8",
   "metadata": {},
   "outputs": [
    {
     "data": {
      "text/latex": [
       "$\\displaystyle 0$"
      ],
      "text/plain": [
       "0"
      ]
     },
     "execution_count": 3,
     "metadata": {},
     "output_type": "execute_result"
    }
   ],
   "source": [
    "import sympy as sm\n",
    "\n",
    "# create symbols for the problem parameters:\n",
    "q = sm.Symbol('q') # mu/L\n",
    "gamma = sm.Symbol('gamma_{k-1}')\n",
    "beta = sm.Symbol('beta_{k-1}')\n",
    "c = sm.Symbol('c_{k-1}')\n",
    "\n",
    "# create symbols for the \"primal\" variables:\n",
    "gk = sm.Symbol('g_{k-1}')\n",
    "dk = sm.Symbol('d_{k-1}')\n",
    "gk1 = sm.Symbol('g_{k}')\n",
    "\n",
    "dk1 = gk1 + beta * dk # define d_{k+1} using previous symbols\n",
    "\n",
    "# inequalities\n",
    "constraint1 = gk1 * dk # == 0\n",
    "constraint2 = dk**2 - c * gk**2 # == 0\n",
    "constraint3 = gk1**2 - beta * gk**2 # == 0\n",
    "\n",
    "lambda1 = 2*beta\n",
    "lambda2 = beta**2 \n",
    "lambda3 = -c * beta \n",
    "\n",
    "# weighted sum\n",
    "weightedSum = lambda1 * constraint1 + lambda2 * constraint2 + lambda3 * constraint3\n",
    "\n",
    "# the weighted sum should be equal to the target reformulation\n",
    "ck1 = (1 + c * beta)\n",
    "\n",
    "target = dk1 ** 2 - ck1 * gk1**2 \n",
    "\n",
    "# Verify that WeightedSum - Target == 0\n",
    "sm.simplify(target-weightedSum)"
   ]
  },
  {
   "cell_type": "code",
   "execution_count": null,
   "id": "d61b31d0-a5ab-477a-b758-cdbd4a052050",
   "metadata": {},
   "outputs": [],
   "source": []
  }
 ],
 "metadata": {
  "kernelspec": {
   "display_name": "Python 3 (ipykernel)",
   "language": "python",
   "name": "python3"
  },
  "language_info": {
   "codemirror_mode": {
    "name": "ipython",
    "version": 3
   },
   "file_extension": ".py",
   "mimetype": "text/x-python",
   "name": "python",
   "nbconvert_exporter": "python",
   "pygments_lexer": "ipython3",
   "version": "3.8.18"
  }
 },
 "nbformat": 4,
 "nbformat_minor": 5
}
